Makefile
@@ -416,7 +416,7 @@ demo931:
 # 	@echo COQC SepApply.v [in-bedrock2-folder]
 # 	@$(COQC) $(COQ_FLAG) -R ../bedrock2/bedrock2/src/bedrock2 bedrock2 -R ../bedrock2/bedrock2/src/exportLogic exportLogic -R ../bedrock2/deps/coqutil/src/coqutil coqutil ../bedrock2/bedrock2/src/exportLogic/SepApply.v
 
-DF=PropositionalLogic/DeepEmbedded/interface_Mendelson.v SeparationLogic/DeepEmbedded/MinimumSeparationLogic_LibSupport.v
+# DF=PropositionalLogic/DeepEmbedded/interface_Mendelson.v SeparationLogic/DeepEmbedded/MinimumSeparationLogic_LibSupport.v
 
 depend:
 	@for name in $(DF); do \
